src/examples/hash_table.v
@@ -1,0 +1,275 @@
+From iris.base_logic.lib Require Import invariants.
+From BurrowLang Require Import lang simp adequacy primitive_laws.
+Require Import Burrow.tpcms.
+Require Import Burrow.ra.
+Require Import Burrow.rollup.
+Require Import Burrow.CpdtTactics.
+Require Import Burrow.tactics.
+
+From iris.base_logic Require Export base_logic.
+From iris.program_logic Require Export weakestpre.
+From iris.proofmode Require Import tactics.
+From iris.program_logic Require Import ectx_lifting.
+From BurrowLang Require Import notation tactics class_instances.
+From BurrowLang Require Import heap_ra.
+From BurrowLang Require Import lang.
+From iris Require Import options.
+
+From Tpcms Require Import hash_table.
+From Tpcms Require Import rwlock.
+From Tpcms Require Import heap.
+From Examples Require Import rwlock.
+From Examples Require Import seqs.
+
+Require Import Burrow.tactics.
+Require Import coq_tricks.Deex.
+
+Definition compute_hash: lang.expr. Admitted.
+
+Definition query_iter: lang.expr :=
+  rec: "query_iter" "slots" "locks" "k" "i" :=
+    if: (BinOp EqOp "i" #(ht_fixed_size)) then
+      PairV #false #()
+    else
+      acquire_shared (seq_idx "i" "locks") ;;
+      let: "ret" := (
+        let: "slot" := ! (seq_idx "i" "slots") in
+          if: (Fst "slot") then
+            let: "k1" := Fst (Snd "slot") in
+            let: "v1" := Snd (Snd "slot") in
+            if: (BinOp EqOp "k" "k1") then
+              Pair #true "v1"
+            else
+              "query_iter" "slots" "locks" "k" ("i" + #1)
+          else
+            PairV #false #()
+      ) in
+      release_shared (seq_idx "i" "locks") ;;
+      "ret"
+.
+
+Definition query: lang.expr :=
+  λ: "query" "ht" "k" ,
+    query_iter (Fst "ht") (Snd "ht") "k" (compute_hash "k").
+
+Section HashTableProof.
+
+Context {𝜇: BurrowCtx}.
+
+Print Instances RelDecision.
+Print Instances Countable.
+
+
+Context `{!simpGS 𝜇 Σ}.
+(*Context `{!HasTPCM 𝜇 (HeapT loc lang.val)}. *)
+
+Context `{!HasTPCM 𝜇 HT}.
+Context `{!HasTPCM 𝜇 (RwLock (HT * (HeapT loc lang.val)))}.
+Context `{!HasRef 𝜇 (rwlock_ref (HT * (HeapT loc lang.val)))}.
+
+Fixpoint seq_iprop (fn: nat -> iProp Σ) (n: nat) :=
+  match n with
+  | 0 => (True)%I
+  | (S i) => (fn i ∗ seq_iprop fn i)%I
+  end.
+
+Lemma get_seq_iprop (fn: nat -> iProp Σ) (n: nat) (i: nat)
+  (i_lt_n : i < n)
+  : seq_iprop fn n ⊢ fn i.
+Proof.
+  induction n.
+  - lia.
+  - have h : Decision (i = n) by solve_decision. destruct h.
+    + subst i. cbn [seq_iprop]. iIntros "[x y]". iFrame.
+    + assert (i < n) by lia. intuition.
+      cbn [seq_iprop]. iIntros "[x y]". iDestruct (H0 with "y") as "y". iFrame.
+Qed.
+
+Instance seq_iprop_persistent fn n (pi: ∀ i , Persistent (fn i)) : Persistent (seq_iprop fn n).
+Proof.
+  induction n.
+  - apply _.
+  - apply _.
+Qed.
+
+Definition slot_as_val (slot: option (Key * Value)) :=
+  match slot with
+  | None => PairV #false #()
+  | Some (k, v) => PairV #true (PairV #k #v)
+  end.
+  
+Definition opt_as_val (val: option Value) :=
+  match val with
+  | None => PairV #false #()
+  | Some v => PairV #true #v
+  end.
+
+Definition ht_inv_i (i: nat) (l: loc) : ((HT * (HeapT loc lang.val)) -> Prop) :=
+  λ p , match p with
+    | (ht, mem) => ∃ slot ,
+      mem = (l $↦ (slot_as_val slot))
+      /\ ht = (s i slot)
+  end.
+
+Definition is_ht_i 𝛾 (slots locks: lang.val) (i: nat) :=
+  match (elem slots i) with
+  | LitV (LitInt l) => (∃ 𝛼 , is_rwlock (elem locks i) 𝛼 𝛾 (ht_inv_i i l))%I
+  | _ => (False) % I
+  end.
+
+Definition is_ht_sl 𝛾 (slots locks: lang.val) :=
+  seq_iprop (is_ht_i 𝛾 slots locks) ht_fixed_size.
+  
+Instance seq_is_ht_sl 𝛾 slots locks : Persistent (is_ht_sl 𝛾 slots locks).
+Proof.
+  apply seq_iprop_persistent.
+  intro. unfold is_ht_i.
+  destruct (elem slots i); try typeclasses eauto.
+  destruct l; typeclasses eauto.
+Qed.
+
+Definition is_ht 𝛾 (ht: lang.val) :=
+  match ht with
+  | PairV slots locks => (is_ht_sl 𝛾 slots locks
+      ∗ ⌜has_length slots ht_fixed_size /\ has_length locks ht_fixed_size⌝
+      )%I
+  | _ => (False)%I
+  end.
+  
+Lemma destruct_slots_i 𝛾 slots locks i
+  : is_ht_i 𝛾 slots locks i -∗ ⌜ ∃ (l: Z) , elem slots i = #l ⌝.
+Proof.
+  iIntros "ih". unfold is_ht_i. destruct (elem slots i).
+  - destruct l.
+    + iPureIntro. exists n. trivial.
+    + iExFalso. iFrame.
+  - iExFalso. iFrame.
+  - iExFalso. iFrame.
+Qed.
+
+Lemma s_i_acquire_shared a : subst "i" a acquire_shared = acquire_shared.
+Proof. trivial. Qed.
+Lemma s_k_acquire_shared a : subst "k" a acquire_shared = acquire_shared.
+Proof. trivial. Qed.
+Lemma s_locks_acquire_shared a : subst "locks" a acquire_shared = acquire_shared.
+Proof. trivial. Qed.
+Lemma s_slots_acquire_shared a : subst "slots" a acquire_shared = acquire_shared.
+Proof. trivial. Qed.
+Lemma s_query_iter_acquire_shared a : subst "query_iter" a acquire_shared = acquire_shared.
+Proof. trivial. Qed.
+Lemma s_i_release_shared a : subst "i" a release_shared = release_shared.
+Proof. trivial. Qed.
+Lemma s_k_release_shared a : subst "k" a release_shared = release_shared.
+Proof. trivial. Qed.
+Lemma s_locks_release_shared a : subst "locks" a release_shared = release_shared.
+Proof. trivial. Qed.
+Lemma s_slots_release_shared a : subst "slots" a release_shared = release_shared.
+Proof. trivial. Qed.
+Lemma s_query_iter_release_shared a : subst "query_iter" a release_shared = release_shared.
+Proof. trivial. Qed.
+Lemma s_i_seq_idx a : subst "i" a seq_idx = seq_idx.
+Proof. trivial. Qed.
+Lemma s_k_seq_idx a : subst "k" a seq_idx = seq_idx.
+Proof. trivial. Qed.
+Lemma s_locks_seq_idx a : subst "locks" a seq_idx = seq_idx.
+Proof. trivial. Qed.
+Lemma s_slots_seq_idx a : subst "slots" a seq_idx = seq_idx.
+Proof. trivial. Qed.
+Lemma s_query_iter_seq_idx a : subst "query_iter" a seq_idx = seq_idx.
+Proof. trivial. Qed.
+
+
+Opaque acquire_shared.
+Opaque release_shared.
+Opaque seq_idx.
+  
+Lemma wp_ht_query 𝜅 𝛾 (slots locks: lang.val) (k: Key) (v: option Value) (i: nat)
+  (i_bound: hash k ≤ i ≤ ht_fixed_size) :
+      {{{ is_ht_sl 𝛾 slots locks ∗ L 𝛾 (m k v) ∗ A 𝜅 ∗ BorrowedRange 𝜅 𝛾 k (hash k) i
+        ∗ ⌜has_length slots ht_fixed_size /\ has_length locks ht_fixed_size⌝ 
+      }}}
+      query_iter slots locks #k #i
+      {{{ RET (opt_as_val v); L 𝛾 (m k v) }}}.
+Proof.
+  iIntros (Phi) "[#ht [m [a [range %szs]]]] Phi".
+  wp_pures.
+    rewrite s_query_iter_acquire_shared.
+    rewrite s_slots_acquire_shared.
+    rewrite s_locks_acquire_shared.
+    rewrite s_k_acquire_shared.
+    rewrite s_i_acquire_shared.
+    rewrite s_query_iter_release_shared.
+    rewrite s_slots_release_shared.
+    rewrite s_locks_release_shared.
+    rewrite s_k_release_shared.
+    rewrite s_i_release_shared.
+    rewrite s_query_iter_seq_idx.
+    rewrite s_slots_seq_idx.
+    rewrite s_locks_seq_idx.
+    rewrite s_k_seq_idx.
+    rewrite s_i_seq_idx.
+  induction i as [i IHi] using (induction_ltof1 _ (λ j, ht_fixed_size - j)); unfold ltof in IHi.
+  unfold query_iter. wp_pures.
+  have h : Decision (i = ht_fixed_size) by solve_decision. destruct h.
+  
+  (* case: i = fixed_size *)
+  
+  - subst i. 
+    assert (bool_decide (#ht_fixed_size = #ht_fixed_size) = true) as bd.
+    { unfold bool_decide. case_decide; crush. }
+    rewrite bd.
+    wp_pures.
+    iDestruct (ht_QueryReachedEnd with "a range m") as "%x". subst v.
+    unfold opt_as_val. iModIntro.
+    iApply "Phi". iFrame.
+  
+  (* case: i < fixed_size *)
+  
+  - 
+    assert (bool_decide (#i = #ht_fixed_size) = false) as bd.
+    { unfold bool_decide. case_decide; trivial. inversion H. lia. }
+    rewrite bd.
+    wp_if.
+    wp_pures.
+    
+    (* lookup lock in sequence *)
+    
+    wp_bind (seq_idx #i locks).
+    wp_apply wp_seq_idx.
+    { apply has_elem_of_has_length with (len := ht_fixed_size).
+      - lia. - intuition. } { done. }
+    iIntros "_".
+    
+    (* acquire lock *)
+    
+    iDestruct (get_seq_iprop _ _ i _ with "ht") as "hti".
+    iDestruct (destruct_slots_i with "hti") as "%ds". 
+    deex. unfold is_ht_i. rewrite ds. iDestruct "hti" as (𝛼) "hti".
+    wp_bind (acquire_shared (elem locks i)).
+    wp_apply (wp_acquire_shared (elem locks i) 𝛼 𝛾 (ht_inv_i i l) with "hti").
+    iIntros (x) "[guard %xinv]".
+    
+    wp_pures. 
+    
+    (* lookup slot ptr in sequence *)
+    
+    wp_bind (seq_idx #i slots).
+    wp_apply wp_seq_idx.
+    { apply has_elem_of_has_length with (len := ht_fixed_size).
+      - lia. - intuition. } { done. }
+    iIntros "_".
+    
+    (* read the slot *)
+    
+    rewrite ds.
+    
+    
+
+Lemma wp_ht_query 𝛾 (ht: lang.val) (k: Key) (v: option Value) :
+      {{{ is_ht 𝛾 ht ∗ L 𝛾 (m k v) }}}
+      query ht #k
+      {{{ RET (opt_as_val v); L 𝛾 (m k v) }}}.
+  
+
+End HashTableProof.
+
